$ (a+b)^n = \binom n 0 a^n + \binom n 1 a^{n-1} b + \binom n 2 a^{n-2} b^2 + \cdots + \binom n k a^{n-k} b^k + \cdots + \binom n n b^n $ 

Pascal's Triangle:
$ \binom n k = \binom {n-1} {k-1} + \binom {n-1} k $ 

Symmetry rule:
$ \binom n k = \binom n {n-k} $

Factoring in:
$ \binom n k = \frac n k \binom {n-1} {k-1} $

Sum over $k$:
$ \sum_{k = 0}^n \binom n k = 2 ^ n $

Sum over $n$:
$ \sum_{m = 0}^n \binom m k = \binom {n + 1} {k + 1} $

Sum over $n$ and $k$:
$ \sum_{k = 0}^m  \binom {n + k} k = \binom {n + m + 1} m $

Sum of the squares:
$ {\binom n 0}^2 + {\binom n 1}^2 + \cdots + {\binom n n}^2 = \binom {2n} n $

Weighted sum:
$ 1 \binom n 1 + 2 \binom n 2 + \cdots + n \binom n n = n 2^{n-1} $

Connection with the Fibonacci numbers:
$ \binom n 0 + \binom {n-1} 1 + \cdots + \binom {n-k} k + \cdots + \binom 0 n = F_{n+1} $

More formulas:
$ \sum_{k=0}^m (-1)^k \cdot \binom{n}{k} = (-1)^m \cdot \binom{n-1}{m} $